src/SmallAlloc.fst
@@ -25,26 +25,26 @@ module G = FStar.Ghost
 //
 //let status : U64.t
 //  = 0UL
-
-let small_alloc
-  (sc: sc)
-  (partial_slabs_ptr empty_slabs_ptr: ref (SL.t blob))
-  : Steel (array U8.t)
-  (SL.ind_llist (p_partial sc) partial_slabs_ptr `star`
-  SL.ind_llist (p_empty sc) empty_slabs_ptr)
-  (fun r ->
-  A.varray r `star`
-  SL.ind_llist (p_partial sc) partial_slabs_ptr `star`
-  SL.ind_llist (p_empty sc) empty_slabs_ptr)
-  (requires fun h0 -> True)
-  (ensures fun h0 r h1 -> True)
-  =
-  //if (U64.eq status 0UL)
-  //then (
-  //  ()
-  //);
-  let r = allocate_slab sc partial_slabs_ptr empty_slabs_ptr (G.hide True) in
-  return r
+let status : U64.t = 0UL
+//let small_alloc
+//  (sc: sc)
+//  (partial_slabs_ptr empty_slabs_ptr: ref (SL.t blob))
+//  : Steel (array U8.t)
+//  (SL.ind_llist (p_partial sc) partial_slabs_ptr `star`
+//  SL.ind_llist (p_empty sc) empty_slabs_ptr)
+//  (fun r ->
+//  A.varray r `star`
+//  SL.ind_llist (p_partial sc) partial_slabs_ptr `star`
+//  SL.ind_llist (p_empty sc) empty_slabs_ptr)
+//  (requires fun h0 -> True)
+//  (ensures fun h0 r h1 -> True)
+//  =
+//  //if (U64.eq status 0UL)
+//  //then (
+//  //  ()
+//  //);
+//  let r = allocate_slab sc partial_slabs_ptr empty_slabs_ptr (G.hide True) in
+//  return r
 
 module L = FStar.List.Tot
 module TLA = Steel.TLArray
